theories/dyn_weak.v
@@ -7,23 +7,29 @@ Unset Strict Implicit.
 Unset Printing Implicit Defensive.
 
 Inductive dyn_agree_ren : (var -> var) ->
-  sta_ctx term -> dyn_ctx term -> sta_ctx term -> dyn_ctx term -> Prop :=
+  sta_ctx -> dyn_ctx -> sta_ctx -> dyn_ctx -> Prop :=
 | dyn_agree_ren_nil ξ :
   dyn_agree_ren ξ nil nil nil nil
 | dyn_agree_ren_ty Γ Γ' Δ Δ' ξ m s :
   dyn_agree_ren ξ Γ Δ Γ' Δ' ->
   dyn_agree_ren (upren ξ)
-    (m :: Γ) (m :{s} Δ) (m.[ren ξ] :: Γ) (m.[ren ξ] :{s} Δ')
+    (m :: Γ) (m :{s} Δ) (m.[ren ξ] :: Γ') (m.[ren ξ] :{s} Δ')
 | dyn_agree_ren_n Γ Γ' Δ Δ' ξ m :
   dyn_agree_ren ξ Γ Δ Γ' Δ' ->
   dyn_agree_ren (upren ξ)
-    (m :: Γ) (_: Δ) (m.[ren ξ] :: Γ) (_: Δ')
+    (m :: Γ) (_: Δ) (m.[ren ξ] :: Γ') (_: Δ')
 | dyn_agree_ren_wkU Γ Γ' Δ Δ' ξ m :
   dyn_agree_ren ξ Γ Δ Γ' Δ' ->
   dyn_agree_ren (ξ >>> (+1)) Γ Δ (m :: Γ') (m :U Δ')
 | dyn_agree_ren_wkN Γ Γ' Δ Δ' ξ m :
   dyn_agree_ren ξ Γ Δ Γ' Δ' ->
   dyn_agree_ren (ξ >>> (+1)) Γ Δ (m :: Γ') (_: Δ').
+
+Lemma dyn_sta_agree_ren Γ Γ' Δ Δ' ξ :
+  dyn_agree_ren ξ Γ Δ Γ' Δ' -> sta_agree_ren ξ Γ Γ'.
+Proof with eauto using sta_agree_ren.
+  elim=>{Γ Γ' Δ Δ' ξ}...
+Qed.
 
 Lemma dyn_agree_ren_refl Γ Δ :
   dyn_wf Γ Δ -> dyn_agree_ren id Γ Δ Γ Δ.
@@ -96,4 +102,78 @@ Proof with eauto 6 using merge, dyn_agree_ren.
   { move=>Γ Γ' Δ Δ' ξ m agr ih Δ1 Δ2 mrg.
     have[Δ1'[Δ2'[mrg'[agr1 agr2]]]]:=ih _ _ mrg.
     exists (_: Δ1'). exists (_: Δ2')... }
+Qed.
+
+Lemma dyn_rename Γ Γ' Δ Δ' m A ξ :
+  Γ ; Δ ⊨ m : A -> dyn_agree_ren ξ Γ Δ Γ' Δ' -> Γ' ; Δ' ⊨ m.[ren ξ] : A.[ren ξ].
+Proof with eauto using dyn_type, dyn_agree_ren, dyn_agree_ren_key.
+  move=>ty. elim: ty Γ' Δ' ξ=>{Γ Δ m A}.
+  { move=>Γ Δ x A shs dhs Γ' Δ' ξ agr. asimpl.
+    apply: dyn_var.
+    apply: sta_agree_ren_has...
+    apply: dyn_sta_agree_ren...
+    apply: dyn_agree_ren_has... }
+  { move=>Γ Δ A B m s t k tyP tym ihm Γ' Δ' ξ agr. asimpl.
+    apply: dyn_lam0...
+    have:=sta_rename tyP (dyn_sta_agree_ren agr).
+    by autosubst. }
+  { move=>Γ Δ A B m s t k tyP tym ihm Γ' Δ' ξ agr. asimpl.
+    apply: dyn_lam1...
+    have:=sta_rename tyP (dyn_sta_agree_ren agr).
+    by autosubst. }
+  { move=>Γ Δ A B m n s t tym ihm tyn Γ' Δ' ξ agr. asimpl.
+    replace B.[n.[ren ξ] .: ren ξ] with B.[ren (upren ξ)].[n.[ren ξ]/]
+      by autosubst.
+    have{}ihm:=ihm _ _ _ agr.
+    have{}ihn:=sta_rename tyn (dyn_sta_agree_ren agr).
+    apply: dyn_app0...
+    asimpl in ihm... }
+  { move=>Γ Δ1 Δ2 Δ A B m n s t mrg tym ihm tyn ihn Γ' Δ' ξ agr. asimpl.
+    replace B.[n.[ren ξ] .: ren ξ] with B.[ren (upren ξ)].[n.[ren ξ]/]
+      by autosubst.
+    have[Δ1'[Δ2'[mrg'[agr1 agr2]]]]:=dyn_agree_ren_merge agr mrg.
+    have{}ihm:=ihm _ _ _ agr1.
+    have{}ihn:=ihn _ _ _ agr2.
+    apply: dyn_app1...
+    asimpl in ihm... }
+  { move=>Γ Δ A B m s eq tym ihm tyB Γ' Δ' ξ agr.
+    apply: dyn_conv.
+    apply: sta_conv_subst...
+    apply: ihm...
+    have:=sta_rename tyB (dyn_sta_agree_ren agr).
+    asimpl... }
+Qed.
+
+Lemma dyn_weakenU Γ Δ m A B :
+  dyn_wf Γ Δ ->
+  Γ ; Δ ⊨ m : A -> (B :: Γ) ; (B :U Δ) ⊨ m.[ren (+1)] : A.[ren (+1)].
+Proof with eauto using dyn_agree_ren, dyn_agree_ren_refl.
+  move=>wf ty. apply: dyn_rename...
+Qed.
+
+Lemma dyn_weakenN Γ Δ m A B :
+  dyn_wf Γ Δ ->
+  Γ ; Δ ⊨ m : A -> (B :: Γ) ; (_: Δ) ⊨ m.[ren (+1)] : A.[ren (+1)].
+Proof with eauto using dyn_agree_ren, dyn_agree_ren_refl.
+  move=>wf ty. apply: dyn_rename...
+Qed.
+
+Lemma dyn_eweakenU Γ Δ m m' A A' B :
+  m' = m.[ren (+1)] ->
+  A' = A.[ren (+1)] ->
+  dyn_wf Γ Δ ->
+  Γ ; Δ ⊨ m : A ->
+  (B :: Γ) ; (B :U Δ) ⊨ m' : A'.
+Proof.
+  move=>*; subst. exact: dyn_weakenU.
+Qed.
+
+Lemma dyn_eweakenN Γ Δ m m' A A' B :
+  m' = m.[ren (+1)] ->
+  A' = A.[ren (+1)] ->
+  dyn_wf Γ Δ ->
+  Γ ; Δ ⊨ m : A ->
+  (B :: Γ) ; (_: Δ) ⊨ m' : A'.
+Proof.
+  move=>*; subst. exact: dyn_weakenN.
 Qed.
