theories/dyn_subst.v
@@ -1,0 +1,40 @@
+From mathcomp Require Import ssreflect ssrbool eqtype ssrnat seq.
+From Coq Require Import ssrfun Classical Utf8.
+Require Export AutosubstSsr ARS sta_subst dyn_weak.
+
+Set Implicit Arguments.
+Unset Strict Implicit.
+Unset Printing Implicit Defensive.
+
+Reserved Notation "Γ1 ; Δ1 ⊨ σ ⫤ Γ2 ; Δ2" (at level 50, σ, Γ2 at next level).
+
+Inductive dyn_agree_subst :
+  context term -> (var -> term) -> context term -> Prop :=
+| agree_subst_nil σ :
+  nil ⊢ σ ⊣ nil
+| agree_subst_ty Δ σ Γ s A :
+  Δ ⊢ σ ⊣ Γ ->
+  A.[σ] :{s} Δ ⊢ up σ ⊣ A :{s} Γ
+| agree_subst_n Δ σ Γ :
+  Δ ⊢ σ ⊣ Γ ->
+  _: Δ ⊢ up σ ⊣ _: Γ
+| agree_subst_wkU Δ σ Γ n A :
+  Δ ⊢ σ ⊣ Γ ->
+  [Δ] ⊢ n : A.[σ] : U ->
+  Δ ⊢ n .: σ ⊣ A :U Γ
+| agree_subst_wkL Δ1 Δ2 Δ σ Γ n A :
+  Δ1 ∘ Δ2 => Δ ->
+  Δ1 ⊢ σ ⊣ Γ ->
+  Δ2 ⊢ n : A.[σ] : L ->
+  Δ ⊢ n .: σ ⊣ A :L Γ
+| agree_subst_wkN Δ σ Γ n :
+  Δ ⊢ σ ⊣ Γ ->
+  Δ ⊢ n .: σ ⊣ _: Γ
+| agree_subst_conv Δ σ Γ A B s l :
+  A <: B ->
+  [Δ] ⊢ B.[ren (+1)].[σ] : s @ l : U ->
+  [Γ] ⊢ B : s @ l : U ->
+  Δ ⊢ σ ⊣ A :{s} Γ ->
+  Δ ⊢ σ ⊣ B :{s} Γ
+where "Δ ⊢ σ ⊣ Γ" := (agree_subst Δ σ Γ).
+
