theories/sta_ctx.v
@@ -1,16 +1,15 @@
 From mathcomp Require Import ssreflect ssrbool eqtype ssrnat seq.
-
 From Coq Require Import ssrfun Classical Utf8.
-Require Import AutosubstSsr ARS.
+Require Import AutosubstSsr ARS tll_ast.
 
 Set Implicit Arguments.
 Unset Strict Implicit.
 Unset Printing Implicit Defensive.
 
-Definition sta_ctx T := seq T.
+Definition sta_ctx := seq term.
 
-Inductive sta_has {T} `{Ids T} `{Subst T} :
-  sta_ctx T -> var -> T -> Prop :=
+Inductive sta_has :
+  sta_ctx -> var -> term -> Prop :=
 | sta_has_O Γ A :
   sta_has (A :: Γ) 0 A.[ren (+1)]
 | sta_has_S Γ A B x :
