theories/tll_ast.v
@@ -1,10 +1,31 @@
 From mathcomp Require Import ssreflect ssrbool eqtype ssrnat seq.
 From Coq Require Import ssrfun Classical Utf8.
-Require Export AutosubstSsr ARS dyn_ctx.
+Require Export AutosubstSsr ARS.
 
 Set Implicit Arguments.
 Unset Strict Implicit.
 Unset Printing Implicit Defensive.
+
+Declare Scope sort_scope.
+Delimit Scope sort_scope with srt.
+Open Scope sort_scope.
+
+Inductive sort : Type := U | L.
+Bind Scope sort_scope with sort.
+
+Definition sort_plus (s t : sort) :=
+  match s with
+  | U => t
+  | L => L
+  end.
+Infix "+" := sort_plus : sort_scope.
+
+Inductive sort_leq : sort -> sort -> Prop :=
+| sort_leqU s :
+  sort_leq U s
+| sort_leqL :
+  sort_leq L L.
+Infix "≤" := sort_leq : sort_scope.
 
 Inductive term : Type :=
 | Var (x : var)
